src/logic/interp.v
@@ -15,11 +15,10 @@ From iris Require Import bi.
 From stdpp Require Import base stringmap fin_map_dom fin_maps.
 
 (* Hazel language *)
-From language Require Import eff_lang.
 From program_logic Require Import protocols weakest_precondition tactics.
 
 (* Local imports *)
-From logic Require Import subst_map.
+From lang Require Import hazel subst_map.
 
 (** * Semantic Types. *)
 
@@ -46,7 +45,7 @@ Section sem_type_interp.
 
   (* Product type. *)
   Definition sem_ty_prod {Σ} (A1 A2 : sem_ty Σ) : sem_ty Σ := 
-    (λ v, ∃ v1 v2, ⌜v = (v1, v2)%V⌝ ∧ A1 v1 ∧ A2 v2)%I.
+    (λ v, ∃ v1 v2, ⌜v = (v1, v2)%V⌝ ∗ A1 v1 ∗ A2 v2)%I.
 
   (* Empty Effect Row. *)
   Definition sem_row_null {Σ} : (sem_row Σ) := iEff_bottom.
@@ -78,70 +77,49 @@ Notation "A ⇒ B" := (sem_row_eff A B)
   (at level 100, B at level 200) : ieff_scope.
 
 
-Section environment.
+Notation ctx Σ := (list (string * (sem_ty Σ))).
 
-  Definition env_sem_typed Σ (Γ : gmap string (sem_ty Σ)) 
-                             (vs : gmap string val) :=
-    (⌜ dom stringset Γ ⊆ dom stringset vs ⌝ ∗ 
-     [∗ map] i ↦ Av ∈ map_zip Γ vs, Av.1 Av.2)%I.
-  
-  Lemma env_sem_typed_lookup Σ Γ vs x A :
-    Γ !! x = Some A →
-    env_sem_typed Σ Γ vs -∗ ∃ v, ⌜ vs !! x = Some v ⌝ ∧ A v.
-  Proof.
-    iIntros (HΓx) "[%Hseq HΓ]".
-    assert (x ∈ (dom stringset vs)).
-    { eapply elem_of_subseteq; first done.
-      apply (elem_of_dom_2 _ _ _ HΓx). }
-    assert (Hsome : is_Some (vs !! x)) by (by apply elem_of_dom).
-    destruct Hsome as [w Hw]. iExists w. iSplitR; first done.
-    iDestruct (big_sepM_lookup _ _ x (A,w) with "HΓ") as "Av"; last done.
-    apply map_lookup_zip_Some; split; done. 
-  Qed.
+(** The domain of the context. *)
+Definition ctx_dom Σ : ctx Σ -> list string := map fst.
 
-  Lemma env_sem_typed_empty Σ : ⊢ env_sem_typed Σ ∅ ∅.
-  Proof. 
-    iIntros "". rewrite /env_sem_typed. iSplit.
-    - iPureIntro. by rewrite !dom_empty. 
-    - by rewrite map_zip_with_empty.
-  Qed.
+Fixpoint env_sem_typed Σ (Γ : ctx Σ)
+                          (vs : gmap string val) : iProp Σ :=
+  match Γ with
+    | [] => True
+    | (x,A) :: Γ' => (∃ v, ⌜ vs !! x = Some v ⌝ ∗ A v) ∗ 
+                          env_sem_typed Σ Γ' vs
+  end.
 
-  Lemma env_sem_typed_insert Σ Γ vs (x : string) A v :
-    A v -∗ env_sem_typed Σ Γ vs -∗
-    env_sem_typed Σ (binder_insert x A Γ) (binder_insert x v vs).
-  Proof.
-    iIntros "HA [%Hdom HΓ]". rewrite /env_sem_typed. iSplit.
-    - rewrite !dom_insert. iPureIntro.
-      by apply union_mono_l.
-    - simpl. rewrite <- map_insert_zip_with. 
-      by iApply (big_sepM_insert_2 with "[HA] HΓ").
-  Qed.
+Lemma env_sem_typed_empty Σ vs : ⊢ env_sem_typed Σ [] vs.
+Proof. done. Qed.
 
-  Lemma env_sem_typed_union Σ Γ₁ Γ₂ vs :
-    Γ₁ ##ₘ Γ₂ →
-    env_sem_typed Σ (Γ₁ ∪ Γ₂) vs ⊢ 
-    (env_sem_typed Σ Γ₁ vs ∗ env_sem_typed Σ Γ₂ vs)%I.
-  Proof. 
-    iIntros (Hdis) "[%Hdom HΓ₁₂]". unfold env_sem_typed.
-    assert (dom stringset Γ₁ ⊆ dom stringset vs ∧ 
-            dom stringset Γ₂ ⊆ dom stringset vs) as [Hdom₁ Hdom₂]. 
-    { apply union_subseteq. by rewrite <- dom_union. }
-    rewrite (bi.sep_comm (⌜dom stringset Γ₂ ⊆ dom stringset vs⌝)%I). 
-    iApply bi.sep_assoc. iSplitL; last (by iPureIntro).
-    iApply bi.sep_assoc. iSplitR; first (by iPureIntro).
-    assert (map_zip (Γ₁ ∪ Γ₂) vs = map_zip Γ₁ vs ∪ map_zip Γ₂ vs) as ->.
-    - admit.
-    - iApply big_sepM_union; last done. 
-      Search "map_disjoint".
-      admit.
-  Admitted.
+Lemma env_sem_typed_insert Σ Γ vs x v :
+  ~In x (ctx_dom Σ Γ) →
+  env_sem_typed Σ Γ vs ⊢ env_sem_typed Σ Γ (binder_insert x v vs).
+Proof.
+  iIntros (HIn) "Henv".
+  iInduction Γ as [|[y A] Γ'] "IH"; first done. simpl in *.
+  iDestruct "Henv" as "((%w & %Hvs & HAw) & HΓ')". iSplitL "HAw".
+  - iExists w. iFrame. iPureIntro.
+    destruct (decide (y = x)) as [->|]. 
+    { destruct HIn. auto. }
+    by rewrite lookup_insert_ne.
+  - iApply "IH"; last done. iPureIntro. tauto.
+Qed.
 
-End environment.
+Lemma env_sem_typed_app Σ Γ₁ Γ₂ vs :
+  env_sem_typed Σ (Γ₁ ++ Γ₂) vs ⊢ 
+  (env_sem_typed Σ Γ₁ vs ∗ env_sem_typed Σ Γ₂ vs)%I.
+Proof. 
+  iIntros "HΓ₁₂". iInduction Γ₁ as [|[y A] Γ₁'] "IH"; first (by iFrame).
+  simpl in *. 
+  iDestruct "HΓ₁₂" as "($ & HΓ₁'₂)". by iApply "IH".
+Qed.
 
 
 (* Semantic typing judgment. *)
 Definition sem_typed `{!irisGS eff_lang Σ}
-  (Γ  : gmap string (sem_ty Σ))
+  (Γ  : ctx Σ)
   (e  : expr)
   (ρ  : sem_row Σ)
   (α  : sem_ty Σ) : Prop :=
@@ -149,6 +127,9 @@ Definition sem_typed `{!irisGS eff_lang Σ}
         env_sem_typed Σ Γ vs ⊢ EWP (subst_map vs e) <| ρ |> {{ α }}.
 
 Notation "Γ ⊨ e : ρ : α" := (sem_typed Γ e ρ α)
+  (at level 74, e, ρ, α at next level) : bi_scope.
+
+Notation "⊨ e : ρ : α" := (sem_typed [] e ρ α)
   (at level 74, e, ρ, α at next level) : bi_scope.
 
 Open Scope bi_scope.
@@ -160,55 +141,123 @@ Open Scope bi_scope.
 Lemma sem_typed_unit `{!irisGS eff_lang Σ} Γ ρ : 
   Γ ⊨ #() : ρ : ().
 Proof.
-  iIntros (vs) "HΓvs //=". by iApply ewp_value.
+  iIntros (vs) "HΓ //=". by iApply ewp_value.
 Qed.
 
 Lemma sem_typed_bool `{!irisGS eff_lang Σ} Γ ρ (b : bool) : 
   Γ ⊨ #b : ρ : 𝔹.
 Proof.
-  iIntros (vs) "HΓvs //=". iApply ewp_value. by iExists b.
+  iIntros (vs) "HΓ //=". iApply ewp_value. by iExists b.
 Qed.
 
 Lemma sem_typed_int `{!irisGS eff_lang Σ} Γ ρ (i : Z) : 
   Γ ⊨ #i : ρ : ℤ.
 Proof.
-  iIntros (vs) "HΓvs //=". iApply ewp_value. by iExists i.
+  iIntros (vs) "HΓ //=". iApply ewp_value. by iExists i.
 Qed.
 
-
 Lemma sem_typed_fun `{!irisGS eff_lang Σ} Γ x e τ ρ κ: 
-  let Γ' := binder_insert x τ Γ in
-  Γ' ⊨ e : ρ : κ →
-  Γ  ⊨ (λ: x, e)%E : ⟨⟩ : (τ -{ ρ }-> κ).
+  ~In x (ctx_dom Σ Γ) →
+  (x,τ) :: Γ ⊨ e : ρ : κ →
+  Γ ⊨ (λ: x, e)%E : ⟨⟩ : (τ -{ ρ }-> κ).
 Proof.
-  iIntros (Γ' He vs) "HΓvs //=".
+  iIntros (HIn He vs) "HΓ //=".
   ewp_pure_steps. iIntros (w) "Hτw". ewp_pure_steps. 
-  destruct x eqn:H; simpl in *.
-  { by iApply He. }
   rewrite <- subst_map_insert.
-  iApply He. unfold Γ'. 
-  iApply (env_sem_typed_insert with "Hτw HΓvs").
+  iApply He. simpl in *. iSplitL "Hτw".
+  - iExists w. iFrame. iPureIntro.
+    by rewrite lookup_insert.
+  - by iApply env_sem_typed_insert.
 Qed.
 
 Lemma sem_typed_app `{!irisGS eff_lang Σ} Γ₁ Γ₂ e₁ e₂ τ ρ κ: 
-  Γ₁ ##ₘ Γ₂ →
   Γ₁ ⊨ e₁ : ρ : (τ -{ ρ }-> κ) →
   Γ₂ ⊨ e₂ : ρ : τ →
-  Γ₁ ∪ Γ₂ ⊨ (e₁ e₂)%E : ρ : κ.
+  Γ₁ ++ Γ₂ ⊨ (e₁ e₂)%E : ρ : κ.
 Proof.
-  iIntros (Hdis He₁ He₂ vs) "HΓ₁₂vs //=".
-  rewrite env_sem_typed_union; last done. 
-  iDestruct "HΓ₁₂vs" as "[HΓ₁vs HΓ₂vs]".
+  iIntros (He₁ He₂ vs) "HΓ₁₂ //=".
+  rewrite env_sem_typed_app.
+  iDestruct "HΓ₁₂" as "[HΓ₁ HΓ₂]".
   iApply (ewp_bind ([AppRCtx (subst_map vs e₁)])); first done.
-  iApply (ewp_mono with "[HΓ₂vs]").
+  iApply (ewp_mono with "[HΓ₂]").
   { by iApply He₂. }
   iIntros (v) "Hτv //=". iModIntro.
   iApply (ewp_bind ([AppLCtx v])); first done.
-  iApply (ewp_mono with "[HΓ₁vs]").
+  iApply (ewp_mono with "[HΓ₁]").
   { by iApply He₁. }
   iIntros (w) "Hτκw //=". iModIntro; by iApply "Hτκw". 
 Qed.
 
-  
+Lemma sem_typed_pair `{!irisGS eff_lang Σ} Γ₁ Γ₂ e₁ e₂ τ ρ κ: 
+  Γ₁ ⊨ e₁ : ρ : τ →
+  Γ₂ ⊨ e₂ : ρ : κ →
+  Γ₁ ++ Γ₂ ⊨ (e₁,e₂)%E : ρ : τ * κ.
+Proof.
+  iIntros (He₁ He₂ vs) "HΓ₁₂ //=".
+  rewrite env_sem_typed_app.
+  iDestruct "HΓ₁₂" as "[HΓ₁ HΓ₂]".
+  iApply (ewp_bind ([PairRCtx (subst_map vs e₁)])); first done.
+  iApply (ewp_mono with "[HΓ₂]").
+  { by iApply He₂. }
+  iIntros (v) "Hτv //=". iModIntro.
+  iApply (ewp_bind ([PairLCtx v])); first done.
+  iApply (ewp_mono with "[HΓ₁]").
+  { by iApply He₁. }
+  iIntros (w) "Hκw //=". iModIntro. ewp_pure_steps.
+  iExists w, v. iFrame. by iPureIntro.
+Qed.
 
+Lemma sem_typed_pair_elim `{!irisGS eff_lang Σ} Γ₁ Γ₂ x₁ x₂ e₁ e₂ τ ρ κ ι: 
+  ~In x₁ (ctx_dom Σ Γ₂) ->
+  ~In x₂ (ctx_dom Σ Γ₂) ->
+  x₁ ≠ x₂ ->
+  Γ₁ ⊨ e₁ : ρ : (τ * κ) →
+  (x₁, τ) :: (x₂, κ) :: Γ₂ ⊨ e₂ : ρ : ι →
+  Γ₁ ++ Γ₂ ⊨ (let: (x₁, x₂) := e₁ in e₂)%E : ρ : ι.
+Proof.
+  iIntros (HIn₁ HIn₂ Hnex₁₂ He₁ He₂ vs) "HΓ₁₂ //=".
+  rewrite env_sem_typed_app.
+  iDestruct "HΓ₁₂" as "[HΓ₁ HΓ₂]".
+  ewp_pure_steps.
+  set ex1x2 := (λ: x₁ x₂, subst_map (binder_delete x₂ 
+                                    (binder_delete x₁ vs)) e₂)%V. 
+  iApply (ewp_bind ([AppLCtx ex1x2])); first done.
+  iApply (ewp_bind ([AppRCtx pair_elim])); first done.
+  iApply (ewp_mono with "[HΓ₁]").
+  { by iApply He₁. }
+  iIntros (v) "Hτκv". iModIntro. simpl in *. 
+  unfold pair_elim. ewp_pure_steps.
+  iDestruct "Hτκv" as "(%v₁ & %v₂ & -> & Hτ & Hκ)".
+  unfold ex1x2. ewp_pure_steps. 
+  destruct (decide _) as [[]|[]]; [|split; [done|congruence]].
+  rewrite delete_commute -subst_map_insert -delete_insert_ne
+    ;last congruence.
+  rewrite <- subst_map_insert.
+  iApply He₂. simpl. iSplitL "Hτ".
+  { iExists v₁. iFrame. iPureIntro. 
+    rewrite lookup_insert_ne; last done.
+    by rewrite lookup_insert. }
+  iSplitL "Hκ".
+  { iExists v₂. iFrame. iPureIntro. 
+    by rewrite lookup_insert. }
+  by repeat (iApply env_sem_typed_insert; first done).
+Qed.
+
+Lemma sem_typed_if `{!irisGS eff_lang Σ} Γ₁ Γ₂ e₁ e₂ e₃ ρ τ: 
+  Γ₁ ⊨ e₁ : ρ : 𝔹 →
+  Γ₂ ⊨ e₂ : ρ : τ →
+  Γ₂ ⊨ e₃ : ρ : τ →
+  Γ₁ ++ Γ₂ ⊨ (if: e₁ then e₂ else e₃)%E : ρ : τ.
+Proof.
+  iIntros (He₁ He₂ He₃ vs) "HΓ₁₂ //=".
+  rewrite env_sem_typed_app.
+  iDestruct "HΓ₁₂" as "[HΓ₁ HΓ₂]".
+  iApply (ewp_bind ([IfCtx (subst_map vs e₂) (subst_map vs e₃)])); first done.
+  iApply (ewp_mono with "[HΓ₁]").
+  { by iApply He₁. }
+  iIntros (v) "(%b & ->)". iModIntro. simpl.
+  destruct b; ewp_pure_steps.
+  - by iApply He₂.
+  - by iApply He₃.
+Qed.
 
