src/lang/hazel.v
@@ -1,0 +1,18 @@
+
+(* Hazel language *)
+From language Require Import eff_lang.
+From program_logic Require Import protocols weakest_precondition tactics.
+
+(* Local imports *)
+From lang Require Import subst_map.
+
+
+Definition pair_elim :=
+  (λ: "x", λ: "f", "f" (Fst "x") (Snd "x"))%V.
+
+Notation ELetPair x1 x2 e1 e2 :=
+  (pair_elim e1 (Lam x1 (Lam x2 e2)))%E.
+
+Notation "'let:' '(' x1 ',' x2 ')' := e1 'in' e2" := (ELetPair x1%binder x2%binder e1%E e2%E)
+  (at level 200, x1, x2 at level 1, e1, e2 at level 200,
+   format "'[' 'let:'  '(' x1 ',' x2 ')'  :=  '[' e1 ']'  'in'  '/' e2 ']'") : expr_scope.
